LivenessValidators.v
@@ -3,27 +3,26 @@ Require Import DecSolve IL Annotation Liveness LengthEq.
 Definition live_sound_dec Lv s slv (an:annotation s slv)
       : Computable (live_sound Lv s slv).
 Proof. 
-  constructor.
   general induction s; destruct slv; try isabsurd.
   + edestruct IHs; eauto; try inv an; eauto;
-    destruct_prop (getAnn slv\{{x}} ⊆ a);
-    destruct_prop (live_exp_sound e a); try dec_solve.
+    decide (getAnn slv\{{x}} ⊆ a);
+    decide (live_exp_sound e a); try dec_solve.
   + edestruct IHs1; try inv an; eauto;
     edestruct IHs2; try inv an; eauto;
-    destruct_prop (x ∈ a); 
-    destruct_prop (getAnn slv1 ⊆ a); 
-    destruct_prop (getAnn slv2 ⊆ a);
+    decide (x ∈ a); 
+    decide (getAnn slv1 ⊆ a); 
+    decide (getAnn slv2 ⊆ a);
     try dec_solve; try eassumption; try inv an; eauto.
   + destruct (get_dec Lv (counted l)) as [[[blv Z] ?]|?];
-    try destruct_prop ((blv \ of_list Z) ⊆ a);
-    destruct_prop (of_list Y ⊆ a);
-    try destruct_prop (length Y = length Z); try dec_solve.
-  +  destruct_prop(x ∈ a); try dec_solve.
+    try decide ((blv \ of_list Z) ⊆ a);
+    decide (of_list Y ⊆ a);
+    try decide (length Y = length Z); try dec_solve.
+  +  decide(x ∈ a); try dec_solve.
   + edestruct IHs1; eauto; try inv an; eauto;
     edestruct IHs2; eauto; try inv an; eauto;
-    destruct_prop ((of_list Z) ⊆ getAnn slv1); 
-    destruct_prop ((getAnn slv1 \ of_list Z) ⊆ a);
-    destruct_prop (getAnn slv2 ⊆ a); try dec_solve.
+    decide ((of_list Z) ⊆ getAnn slv1); 
+    decide ((getAnn slv1 \ of_list Z) ⊆ a);
+    decide (getAnn slv2 ⊆ a); try dec_solve.
     Grab Existential Variables. eassumption. eassumption.
 Defined.
 
@@ -31,44 +30,43 @@ Defined.
 Instance live_sound_dec_inst Lv s slv `{Computable(annotation s slv)}
 : Computable (live_sound Lv s slv).
 Proof.
-  destruct H as [[]].
+  edestruct H.
   eapply live_sound_dec; eauto.
-  constructor. right; intro. eauto using live_sound_annotation.
+  right; intro. eauto using live_sound_annotation.
 Defined.
 
 Definition true_live_sound_dec Lv s slv (an:annotation s slv)
       : Computable (true_live_sound Lv s slv).
 Proof. 
-  constructor.
   general induction s; destruct slv; try isabsurd.
   + edestruct IHs; eauto; try inv an; eauto;
-    destruct_prop (getAnn slv\{{x}} ⊆ a);
-    destruct_prop (x ∈ getAnn slv -> live_exp_sound e a); 
-(*    destruct_prop (x ∉ getAnn slv -> a ⊆ getAnn slv\{{x}});*) try dec_solve. 
+    decide (getAnn slv\{{x}} ⊆ a);
+    decide (x ∈ getAnn slv -> live_exp_sound e a); 
+(*    decide (x ∉ getAnn slv -> a ⊆ getAnn slv\{{x}});*) try dec_solve. 
   + edestruct IHs1; try inv an; eauto;
     edestruct IHs2; try inv an; eauto;
-    destruct_prop (x ∈ a); 
-    destruct_prop (getAnn slv1 ⊆ a); 
-    destruct_prop (getAnn slv2 ⊆ a);
+    decide (x ∈ a); 
+    decide (getAnn slv1 ⊆ a); 
+    decide (getAnn slv2 ⊆ a);
     try dec_solve; try eassumption; try inv an; eauto.
   + destruct (get_dec Lv (counted l)) as [[[blv Z] ?]|?];
-    try destruct_prop ((blv \ of_list Z) ⊆ a);
-    try destruct_prop (argsLive a blv Y Z); try dec_solve.
+    try decide ((blv \ of_list Z) ⊆ a);
+    try decide (argsLive a blv Y Z); try dec_solve.
     left. econstructor; eauto using argsLive_length.
-  + destruct_prop(x ∈ a); try dec_solve.
+  + decide(x ∈ a); try dec_solve.
   + edestruct IHs1; eauto; try inv an; eauto;
     edestruct IHs2; eauto; try inv an; eauto;
-    destruct_prop ((getAnn slv1 \ of_list Z) ⊆ a);
-    destruct_prop (getAnn slv2 ⊆ a); try dec_solve.
+    decide ((getAnn slv1 \ of_list Z) ⊆ a);
+    decide (getAnn slv2 ⊆ a); try dec_solve.
     Grab Existential Variables. eassumption. eassumption.
 Defined.
 
 Instance true_live_sound_dec_inst Lv s slv `{Computable(annotation s slv)}
 : Computable (true_live_sound Lv s slv).
 Proof.
-  destruct H as [[]].
+  edestruct H.
   eapply true_live_sound_dec; eauto.
-  constructor. right; intro. eauto using true_live_sound_annotation.
+  right; intro. eauto using true_live_sound_annotation.
 Defined.
 
 (* 
